try switch to different gc

src/Gc.v
@@ -1,5 +1,6 @@
 Require Import Gc.Language.
 Require Import List ListSet Equality CpdtTactics.
+Require Import Coq.Program.Wf.
 
 Inductive addresing_string : Type :=
 | TermStr : addresing_string
@@ -27,6 +28,52 @@ Fixpoint union_pointers (l : list (set ptr)) : set ptr :=
   | nil => (empty_set ptr)
   | h::t => (set_union ptr_eq_dec h  (union_pointers t))
   end.
+
+Theorem union_pointers_nodup :
+  forall l,
+    Forall (fun a => NoDup a) l ->
+    NoDup (union_pointers l).
+Proof.
+  intros.
+  induction l.
+  constructor.
+  eapply set_union_nodup ;
+    inversion H ;
+    eauto.
+Qed.
+
+Theorem set_union_nodup_inv_1 :
+  forall l l',
+    NoDup (set_union ptr_eq_dec l l') ->
+    NoDup l.
+Proof.
+  intros l l'. revert l.
+  induction l'.
+  * intros.
+    induction l; crush.
+  * intros.
+    unfold set_union in * ; fold set_union in *.
+    specialize (IHl' l).
+    induction (((fix set_union (x y : set nat) {struct y} : set nat :=
+               match y with
+               | nil => x
+               | a1 :: y1 => set_add ptr_eq_dec a1 (set_union x y1)
+               end) l l')).
+  - eapply IHl'. constructor.
+  - crush.
+    destruct (ptr_eq_dec a a0).
+    + eauto.
+    + inversion H. subst.
+      assert (NoDup s -> NoDup l).
+      ** intros.
+         assert (~ In a0 s).
+         unfold not. intros.
+         assert (In a0 (set_add ptr_eq_dec a s)). eapply set_add_intro1; auto.
+         crush.
+         assert (NoDup (a0 :: s)). constructor ; auto.
+         intuition.
+      ** eauto.
+Qed.
 
 Theorem nth_union_pointers:
   forall l n p,
@@ -63,21 +110,283 @@ Proof.
     crush.
 Qed.
 
+Lemma heap_get_to_maps :
+  forall h p v,
+    heap_get_struct p h = Some v ->
+    In (p,v) h.
+Proof.
+  induction h. crush.
+  intros.
+  unfold heap_get_struct in H.
+  destruct a.
+  edestruct ptr_eq_dec eqn:?. constructor. injection H. intros. subst. reflexivity.
+  crush.
+Qed.
+
+Lemma heap_get_to_maps_2 :
+  forall h p v,
+    heap_get_struct p h = Some v ->
+    In p (fst (split h)).
+Proof.
+  intros.
+  specialize (heap_get_to_maps _ _ _ H).
+  intros.
+  unfold set_In in *. unfold ptr in *.
+  assert (p = fst (p,v)). crush. rewrite H1. clear H1.
+  eapply in_split_l. auto.
+Qed.
+
+
+Theorem set_add_noop :
+  forall l a,
+    set_In a l ->
+    set_add ptr_eq_dec a l = l.
+Proof.
+  induction l. crush.
+  intros.
+  unfold set_In in *. unfold In in *.
+  destruct H.
+  * subst. unfold set_add. destruct (ptr_eq_dec a0 a0) eqn:? ; crush.
+  * crush. edestruct ptr_eq_dec ; reflexivity.
+Qed.
+
 Fixpoint mark_ptr (fuel:nat) (p: ptr) (h: heap_t) : set ptr :=
   match fuel, heap_get_struct p h with
   | S n, Some vs =>
     (set_add ptr_eq_dec p
-        (union_pointers
-           (List.map
-              (fun v =>
-                 match v with
-                 | Int _ => nil
-                 | Pointer p' => mark_ptr n p' h
-                 end
-              ) vs)))
+             (union_pointers
+                (List.map
+                   (fun v =>
+                      match v with
+                      | Int _ => nil
+                      | Pointer p' => mark_ptr n p' h
+                      end
+                   ) vs)))
   | _, _ => nil
   end
 .
+
+Definition add_vals (h: heap_t) (p: ptr) : set ptr :=
+  nodup
+    ptr_eq_dec
+    match heap_get_struct p h with
+    | Some vs =>
+      (List.flat_map
+         (fun v =>
+            match v with
+            | Int _ => nil
+            | Pointer p' =>
+              match heap_get_struct p' h with
+              | Some _ => p'::nil
+              | None => nil
+              end
+            end
+         ) vs)
+    | None => nil
+    end.
+
+Theorem add_vals_subset :
+  forall h p p',
+    set_In p' (add_vals h p) ->
+    In p' (fst (split h)).
+Proof.
+  intros.
+  unfold add_vals in H.
+  destruct (heap_get_struct p h) eqn:?. Focus 2. crush.
+  clear Heqo.
+  induction l. crush.
+  unfold flat_map in H ; fold flat_map in H.
+  destruct a.
+  remember (((fix flat_map (l : list val) : list ptr :=
+               match l with
+               | nil => nil
+               | x :: t =>
+                   match x with
+                   | Int _ => nil
+                   | Pointer p' =>
+                       match heap_get_struct p' h with
+                       | Some _ => p' :: nil
+                       | None => nil
+                       end
+                   end ++ flat_map t
+               end) l)) as foo.
+  specialize (app_nil_l foo).
+  intros. rewrite H0 in H. clear H0. rewrite Heqfoo in H. intuition.
+  destruct (heap_get_struct p0 h) eqn:?.
+  * unfold app in H.
+    unfold nodup in H.
+    destruct (in_dec ptr_eq_dec p0).
+    - intuition.
+    - crush.
+      eapply heap_get_to_maps_2. apply Heqo.
+  * crush.
+Qed.
+
+Fixpoint mark_ptr_single (h: heap_t) (ps: set ptr) : set ptr :=
+  match ps with
+  | nil => nil
+  | p::ps' =>
+    set_add
+      ptr_eq_dec
+      p
+      (set_union
+         ptr_eq_dec
+         (add_vals h p)
+         (mark_ptr_single h ps')
+      )
+  end.
+
+Theorem mark_ptr_single_nodup :
+  forall h ps,
+    NoDup ps ->
+    NoDup (mark_ptr_single h ps).
+Proof.
+  induction ps. crush.
+  intros. inversion H. subst. intuition.
+  unfold mark_ptr_single. fold mark_ptr_single.
+  eapply set_add_nodup.
+  eapply set_union_nodup ; auto.
+  unfold add_vals. eapply NoDup_nodup.
+Qed.
+
+Theorem mark_ptr_single_monotonic_1 :
+  forall h p ps,
+    NoDup ps ->
+    In p ps ->
+    In p (mark_ptr_single h ps).
+Proof.
+  intros until ps. revert h p.
+  induction ps. crush.
+  intros.
+  inversion H. clear H. subst.
+  specialize (IHps h p H4).
+  destruct H0. subst.
+  * unfold mark_ptr_single. fold mark_ptr_single.
+    eapply set_add_intro2. reflexivity.
+  * unfold mark_ptr_single. fold mark_ptr_single.
+    eapply set_add_intro1.
+    eapply set_union_intro2.
+    intuition.
+Qed.
+
+Theorem mark_ptr_single_monotonic_2 :
+  forall h ps,
+    NoDup ps ->
+    incl ps (mark_ptr_single h ps).
+Proof.
+  unfold incl.
+  intros.
+  eapply mark_ptr_single_monotonic_1 ; auto.
+Qed.
+
+Lemma incl_cons_inv :
+  forall {A: Type} (a: A) b c,
+    incl (a::b) c ->
+    incl b c.
+Proof.
+  intros until c. generalize a c.
+  induction b ; induction c ; crush.
+  * unfold incl. intros. inversion H0.
+  * unfold incl in *.
+    intros.
+    specialize (H a2).
+    assert (In a2 (a1 :: a0 :: b)). crush. intuition.
+Qed.
+
+
+Lemma mark_ptr_single_subset_1 :
+  forall h ps p,
+    NoDup ps ->
+    incl ps (fst (split h)) ->
+    set_In p (mark_ptr_single h ps) ->
+    set_In p (fst (split h)).
+Proof.
+  induction ps. crush.
+  intros. inversion H. subst. clear H.
+  assert (incl ps (fst (split h))). eapply incl_cons_inv. apply H0.
+  specialize (IHps p H5 H).
+  unfold mark_ptr_single in * ; fold mark_ptr_single in *.
+  destruct (set_add_elim _ _ _ _ H1) ; clear H1. crush. eapply incl_cons_inv ; crush.
+  destruct (set_union_elim _ _ _ _ H2) ; clear H2.
+  * eapply add_vals_subset. apply H1.
+  * crush.
+Qed.
+
+Lemma mark_ptr_single_subset_2 :
+  forall h ps,
+    NoDup ps ->
+    incl ps (fst (split h)) ->
+    incl (mark_ptr_single h ps) (fst (split h)).
+Proof.
+  unfold incl.
+  intros.
+  eapply mark_ptr_single_subset_1. apply H. auto. auto.
+Qed.
+
+Lemma mark_ptr_single_subset_3 :
+  forall h ps,
+    NoDup ps ->
+    incl ps (fst (split h)) ->
+    length (mark_ptr_single h ps) <= length (fst (split h)).
+Proof.
+  intros.
+  eapply NoDup_incl_length.
+  eapply mark_ptr_single_nodup. auto.
+  eapply mark_ptr_single_subset_2. auto. auto.
+Qed.
+
+Program Fixpoint mark_ptr_full' (h: heap_t) (ps: set ptr) (H: NoDup ps) (H': incl ps (fst (split h)))
+        {measure (length h - length ps)} : set ptr :=
+  let new := mark_ptr_single h ps in
+  if PeanoNat.Nat.eq_dec (length ps) (length new)
+  then
+    new
+  else
+    mark_ptr_full' h new _ _
+.
+Next Obligation.
+  clear H0.
+  eapply mark_ptr_single_nodup. auto.
+Defined.
+Next Obligation.
+  eapply mark_ptr_single_subset_2 ; auto.
+Defined.
+Next Obligation.
+  clear mark_ptr_full'.
+
+  assert (length ps > 0).
+  destruct ps ; crush.
+
+  assert (length (mark_ptr_single h ps) >= length ps).
+  assert (incl ps (mark_ptr_single h ps)).
+  eapply mark_ptr_single_monotonic_2 ; auto.
+  eapply NoDup_incl_length ; auto.
+
+  assert (length (mark_ptr_single h ps) > length ps).
+  crush.
+
+  assert (length (mark_ptr_single h ps) <= length h).
+  specialize (mark_ptr_single_subset_3 _ _ H H').
+  intros.
+  specialize (split_length_l h). intros. crush.
+
+  assert (length ps < length h) ; crush.
+Defined.
+
+Program Definition mark_ptr_full (r: roots_t) (h: heap_t) : set ptr :=
+  let root_ptrs := (snd (split r)) in
+  let present_root_ptrs := set_inter ptr_eq_dec root_ptrs (fst (split h)) in
+  mark_ptr_full' h (nodup ptr_eq_dec present_root_ptrs) _ _
+.
+Next Obligation.
+  eapply NoDup_nodup.
+Defined.
+Next Obligation.
+  unfold incl. intros.
+  specialize (nodup_In ptr_eq_dec (set_inter ptr_eq_dec (snd (split r)) (fst (split h))) a). intros. destruct H0.
+  intuition. clear - H2.
+  destruct (set_inter_elim _ _ _ _ H2) ; auto.
+Defined.
 
 Theorem mark_ptr_subset:
   forall f e p h,
@@ -104,18 +413,18 @@ Proof.
                      | Int _ => nil
                      | Pointer p' => mark_ptr f p' h
                      end) l (Int 0) x).
-  unfold ptr. unfold set.
-  unfold ptr in H. unfold set in H.
-  intros. rewrite H0 in H. clear H0.
-  destruct (nth x l (Int 0)). crush.
-  eapply IHf. apply H.
+    unfold ptr. unfold set.
+    unfold ptr in H. unfold set in H.
+    intros. rewrite H0 in H. clear H0.
+    destruct (nth x l (Int 0)). crush.
+    eapply IHf. apply H.
   * crush.
 Qed.
 
 Theorem mark_ptr_monotonic_1 :
   forall f e p h,
-  set_In e (mark_ptr f p h) ->
-  set_In e (mark_ptr (S f) p h).
+    set_In e (mark_ptr f p h) ->
+    set_In e (mark_ptr (S f) p h).
 Proof.
   induction f. crush.
   intros.
@@ -136,22 +445,22 @@ Proof.
                 val
                 (list ptr)
                 (fun v : val =>
-           match v with
-           | Int _ => nil
-           | Pointer p' =>
-               match heap_get_struct p' h with
-               | Some vs =>
-                   set_add ptr_eq_dec p'
-                     (union_pointers
-                        (map
-                           (fun v0 : val =>
-                            match v0 with
-                            | Int _ => nil
-                            | Pointer p'0 => mark_ptr f p'0 h
-                            end) vs))
-               | None => nil
-               end
-           end) l (Int 0) x).
+                   match v with
+                   | Int _ => nil
+                   | Pointer p' =>
+                     match heap_get_struct p' h with
+                     | Some vs =>
+                       set_add ptr_eq_dec p'
+                               (union_pointers
+                                  (map
+                                     (fun v0 : val =>
+                                        match v0 with
+                                        | Int _ => nil
+                                        | Pointer p'0 => mark_ptr f p'0 h
+                                        end) vs))
+                     | None => nil
+                     end
+                   end) l (Int 0) x).
   unfold ptr. unfold set.
   intros. rewrite H0. clear H0.
 
@@ -159,10 +468,10 @@ Proof.
                 val
                 (list ptr)
                 (fun v : val =>
-                match v with
-                | Int _ => nil
-                | Pointer p' => mark_ptr f p' h
-                end) l (Int 0) x).
+                   match v with
+                   | Int _ => nil
+                   | Pointer p' => mark_ptr f p' h
+                   end) l (Int 0) x).
   unfold ptr. unfold set.
   unfold ptr in H1. unfold set in H1.
   intros. rewrite H0 in H1. clear H0.
@@ -184,10 +493,10 @@ Proof.
   * intros.
     specialize (IHf' e p h). intuition.
     inversion H0.
-    - subst. auto.
-    - intuition.
-      eapply mark_ptr_monotonic_1.
-      auto.
+  - subst. auto.
+  - intuition.
+    eapply mark_ptr_monotonic_1.
+    auto.
 Qed.
 
 Theorem mark_ptr_monotonic_3 :
@@ -220,39 +529,39 @@ Proof.
     inversion H0. clear H0.
     subst.
     induction h.
-    - inversion H.
-    - assert (length (a :: h) = S (length h)) ; auto.
-      rewrite H0.
-      unfold mark_ptr.
-      rewrite H.
-      apply set_add_iff; crush.
-  * intros.
-    inversion H.
-    subst.
-    specialize (IHaddress h p'0 p' H6).
-    assert (set_In p' (mark_ptr (S (length h)) p h)).
-    - unfold mark_ptr ; fold mark_ptr.
-      specialize (heap_maps_implies_heap_get h p n (Pointer p'0) H4).
-      intros. destruct H0. destruct H0.
-      rewrite H0.
-      eapply set_add_intro1.
-      eapply (nth_union_pointers _ n).
+  - inversion H.
+  - assert (length (a :: h) = S (length h)) ; auto.
+    rewrite H0.
+    unfold mark_ptr.
+    rewrite H.
+    apply set_add_iff; crush.
+    * intros.
+      inversion H.
+      subst.
+      specialize (IHaddress h p'0 p' H6).
+      assert (set_In p' (mark_ptr (S (length h)) p h)).
+  - unfold mark_ptr ; fold mark_ptr.
+    specialize (heap_maps_implies_heap_get h p n (Pointer p'0) H4).
+    intros. destruct H0. destruct H0.
+    rewrite H0.
+    eapply set_add_intro1.
+    eapply (nth_union_pointers _ n).
 
-      specialize (@map_nth
-                    val
-                    (list ptr)
-                    (fun v : val =>
-                       match v return list ptr with
-                       | Int _ => nil
-                       | Pointer p'1 => mark_ptr (length h) p'1 h
+    specialize (@map_nth
+                  val
+                  (list ptr)
+                  (fun v : val =>
+                     match v return list ptr with
+                     | Int _ => nil
+                     | Pointer p'1 => mark_ptr (length h) p'1 h
                      end) x (Int 0) n).
-      intros. rewrite H2 ; clear H2.
-      specialize (nth_default_eq n x (Int 0)). intros.
-      rewrite <- H2. intros. clear H2.
-      unfold nth_default. rewrite H1.
-      auto.
-    - eapply mark_ptr_saturates.
-      apply H0.
+    intros. rewrite H2 ; clear H2.
+    specialize (nth_default_eq n x (Int 0)). intros.
+    rewrite <- H2. intros. clear H2.
+    unfold nth_default. rewrite H1.
+    auto.
+  - eapply mark_ptr_saturates.
+    apply H0.
 Qed.
 
 Theorem mark_ptr_correct :
@@ -281,24 +590,24 @@ Proof.
     * crush.
       eauto.
     * dependent induction l.
-      + crush.
-      + rewrite map_cons in H.
-        destruct a eqn:?.
-        -- crush.
-           apply set_union_emptyL in H.
-           eauto.
-        -- simpl in H.
-           apply set_union_iff in H.
-           destruct H.
-           ** specialize IHf with p0.
-              intuition.
-              edestruct H2.
-              assert (exists k, heap_maps h p k a).
-              ++ crush.
-              ++ edestruct H4.
-                 exists (FollowStr x0 x).
-                 eapply (FollowAddresses h p p0 p'); subst; eauto.
-           ** apply IHl; intuition.
+    + crush.
+    + rewrite map_cons in H.
+      destruct a eqn:?.
+      -- crush.
+         apply set_union_emptyL in H.
+         eauto.
+      -- simpl in H.
+         apply set_union_iff in H.
+         destruct H.
+         ** specialize IHf with p0.
+            intuition.
+            edestruct H2.
+            assert (exists k, heap_maps h p k a).
+         ++ crush.
+         ++ edestruct H4.
+            exists (FollowStr x0 x).
+            eapply (FollowAddresses h p p0 p'); subst; eauto.
+            ** apply IHl; intuition.
 Qed.
 
 Fixpoint mark (r: roots_t) (h: heap_t) : set ptr :=
@@ -341,17 +650,17 @@ Proof.
     unfold roots_maps in *.
     specialize (in_inv H). intros.
     destruct H1.
-    - clear H. injection H1. clear H1. intros. subst.
-      unfold mark. fold mark.
-      specialize (mark_ptr_marks address h p p' H0).
-      intros.
-      eapply set_union_intro2. auto.
-    - intuition.
+  - clear H. injection H1. clear H1. intros. subst.
+    unfold mark. fold mark.
+    specialize (mark_ptr_marks address h p p' H0).
+    intros.
+    eapply set_union_intro2. auto.
+  - intuition.
+    crush.
+    + apply set_union_iff.
       crush.
-      + apply set_union_iff.
-        crush.
-      + apply set_union_iff.
-        crush.
+    + apply set_union_iff.
+      crush.
 Qed.
 
 Lemma address_extend :
@@ -393,156 +702,156 @@ Proof.
     unfold heap_maps_struct in * ; fold heap_maps_struct in *.
     unfold heap_get_struct in * ; fold heap_get_struct in *.
     destruct (ptr_eq_dec p p') eqn:?.
-    - crush.
-      assert (set_mem ptr_eq_dec p' foo = true). eapply set_mem_correct2. auto.
-      rewrite H.
-      constructor. exists x. unfold heap_maps_struct. unfold heap_get_struct.
-      destruct (ptr_eq_dec p' p'). crush. crush.
-    - destruct (set_mem ptr_eq_dec p foo).
-      + crush.
-        inversion H1. destruct H2. subst.
-        constructor. exists x0.
-        unfold heap_maps_struct. unfold heap_get_struct.
-        destruct (ptr_eq_dec p p'). crush. crush.
-      + crush.
-  * crush.
-    inversion H. clear H. subst.
-    specialize (IHaddress r h p'0 p' H7).
-    assert (set_In p'0 (mark r h)).
-    - clear IHaddress.
-      induction r. crush.
-      destruct a.
-      destruct (ptr_eq_dec p'0 p0) eqn:?.
-      + crush.
-        assert (exists x, length h = S x). destruct h. unfold heap_maps in H5. unfold heap_get in H5. crush. exists (length h). crush.
-        destruct H. rewrite H. unfold mark_ptr. fold mark_ptr.
-        clear H Heqs IHr H0 H5.
-        eapply set_union_intro2.
-        inversion H7.
-        ** destruct H. subst.
-           rewrite H. eapply set_add_intro2. auto.
-        ** subst.
-           unfold heap_maps in H. unfold heap_get in H.
-           destruct (heap_get_struct p0 h). Focus 2. crush.
-           eapply set_add_intro2. auto.
-      + unfold mark in * ; fold mark in *.
-        unfold set_In in *.
-        destruct (set_union_elim _ _ _ _ H0).
-        ** crush. eapply set_union_intro1. auto.
-        ** specialize (mark_ptr_correct _ _ _ _ H).
-           intros.
-           destruct H1.
-           inversion H7.
-           -- subst. clear H7.
-              destruct H2.
-              specialize (set_union_elim _ _ _ _ H0). intros. clear H0.
-              destruct H3.
-              ++ intuition.
-                 eapply set_union_intro1. auto.
-              ++ eapply set_union_intro2. auto.
-                 destruct (ptr_eq_dec p' p). crush.
-                 assert (exists x, length h = S (S x)). destruct h. crush.
-                 destruct h.
-                 *** destruct p1.
-                     assert (p1 = p).
-                     --- unfold heap_maps in H5.
-                         unfold heap_get in H5.
-                         unfold heap_get_struct in H5.
-                         destruct (ptr_eq_dec p1 p). crush. crush.
-                     --- assert (p1 = p').
-                         unfold heap_maps_struct in H2.
-                         unfold heap_get_struct in H2.
-                         destruct (ptr_eq_dec p1 p'). crush. crush.
-                         crush.
-                 *** exists (length h). auto.
-                 *** destruct H3. rewrite H3 in H0.
-                     destruct (heap_get_struct p0 h) eqn:?.
-                     --- unfold mark_ptr in H0. fold mark_ptr in H0.
-                         rewrite Heqo in H0.
-                         specialize (set_add_elim _ _ _ _ H0).
-                         intros. destruct H4 ; subst.
-                         +++ rewrite H3.
-                             unfold mark_ptr in *. fold mark_ptr in *.
-                             rewrite Heqo.
-                             eapply set_add_intro1.
-                             eapply (nth_union_pointers _ n).
-                             unfold heap_maps in H5.
-                             unfold heap_get in H5.
-                             rewrite Heqo in H5.
-                             specialize (@map_nth
-                                           val
-                                           (list ptr)
-                                           (fun v : val =>
-                                              match v with
-                                              | Int _ => nil
-                                              | Pointer p'0 =>
-                                                match heap_get_struct p'0 h with
-                                                | Some vs =>
-                                                  set_add ptr_eq_dec p'0
-                                                          (union_pointers
-                                                             (map
-                                                                (fun v0 : val =>
-                                                                   match v0 with
-                                                                   | Int _ => nil
-                                                                   | Pointer p'1 => mark_ptr x1 p'1 h
-                                                                   end) vs))
-                                                | None => nil
-                                                end
-                                              end) l (Int 0) n).
-                             intros.
-                             unfold ptr in *. unfold set in *.
-                             rewrite H4. clear H4.
-                             specialize (nth_default_eq n l (Int 0)). intros.
-                             rewrite <- H4.
-                             unfold nth_default.
-                             rewrite H5.
-                             destruct x1.
-                             **** unfold heap_maps_struct in H2.
-                                  rewrite H2.
-                                  eapply set_add_intro2. reflexivity.
-                             **** crush.
-                                  eapply set_add_intro2. reflexivity.
-                         +++ clear H0.
+  - crush.
+    assert (set_mem ptr_eq_dec p' foo = true). eapply set_mem_correct2. auto.
+    rewrite H.
+    constructor. exists x. unfold heap_maps_struct. unfold heap_get_struct.
+    destruct (ptr_eq_dec p' p'). crush. crush.
+  - destruct (set_mem ptr_eq_dec p foo).
+    + crush.
+      inversion H1. destruct H2. subst.
+      constructor. exists x0.
+      unfold heap_maps_struct. unfold heap_get_struct.
+      destruct (ptr_eq_dec p p'). crush. crush.
+    + crush.
+      * crush.
+        inversion H. clear H. subst.
+        specialize (IHaddress r h p'0 p' H7).
+        assert (set_In p'0 (mark r h)).
+  - clear IHaddress.
+    induction r. crush.
+    destruct a.
+    destruct (ptr_eq_dec p'0 p0) eqn:?.
+    + crush.
+      assert (exists x, length h = S x). destruct h. unfold heap_maps in H5. unfold heap_get in H5. crush. exists (length h). crush.
+      destruct H. rewrite H. unfold mark_ptr. fold mark_ptr.
+      clear H Heqs IHr H0 H5.
+      eapply set_union_intro2.
+      inversion H7.
+      ** destruct H. subst.
+         rewrite H. eapply set_add_intro2. auto.
+      ** subst.
+         unfold heap_maps in H. unfold heap_get in H.
+         destruct (heap_get_struct p0 h). Focus 2. crush.
+         eapply set_add_intro2. auto.
+    + unfold mark in * ; fold mark in *.
+      unfold set_In in *.
+      destruct (set_union_elim _ _ _ _ H0).
+      ** crush. eapply set_union_intro1. auto.
+      ** specialize (mark_ptr_correct _ _ _ _ H).
+         intros.
+         destruct H1.
+         inversion H7.
+      -- subst. clear H7.
+         destruct H2.
+         specialize (set_union_elim _ _ _ _ H0). intros. clear H0.
+         destruct H3.
+         ++ intuition.
+            eapply set_union_intro1. auto.
+         ++ eapply set_union_intro2. auto.
+            destruct (ptr_eq_dec p' p). crush.
+            assert (exists x, length h = S (S x)). destruct h. crush.
+            destruct h.
+            *** destruct p1.
+                assert (p1 = p).
+            --- unfold heap_maps in H5.
+                unfold heap_get in H5.
+                unfold heap_get_struct in H5.
+                destruct (ptr_eq_dec p1 p). crush. crush.
+            --- assert (p1 = p').
+                unfold heap_maps_struct in H2.
+                unfold heap_get_struct in H2.
+                destruct (ptr_eq_dec p1 p'). crush. crush.
+                crush.
+                *** exists (length h). auto.
+                *** destruct H3. rewrite H3 in H0.
+                    destruct (heap_get_struct p0 h) eqn:?.
+            --- unfold mark_ptr in H0. fold mark_ptr in H0.
+                rewrite Heqo in H0.
+                specialize (set_add_elim _ _ _ _ H0).
+                intros. destruct H4 ; subst.
+                +++ rewrite H3.
+                    unfold mark_ptr in *. fold mark_ptr in *.
+                    rewrite Heqo.
+                    eapply set_add_intro1.
+                    eapply (nth_union_pointers _ n).
+                    unfold heap_maps in H5.
+                    unfold heap_get in H5.
+                    rewrite Heqo in H5.
+                    specialize (@map_nth
+                                  val
+                                  (list ptr)
+                                  (fun v : val =>
+                                     match v with
+                                     | Int _ => nil
+                                     | Pointer p'0 =>
+                                       match heap_get_struct p'0 h with
+                                       | Some vs =>
+                                         set_add ptr_eq_dec p'0
+                                                 (union_pointers
+                                                    (map
+                                                       (fun v0 : val =>
+                                                          match v0 with
+                                                          | Int _ => nil
+                                                          | Pointer p'1 => mark_ptr x1 p'1 h
+                                                          end) vs))
+                                       | None => nil
+                                       end
+                                     end) l (Int 0) n).
+                    intros.
+                    unfold ptr in *. unfold set in *.
+                    rewrite H4. clear H4.
+                    specialize (nth_default_eq n l (Int 0)). intros.
+                    rewrite <- H4.
+                    unfold nth_default.
+                    rewrite H5.
+                    destruct x1.
+                    **** unfold heap_maps_struct in H2.
+                         rewrite H2.
+                         eapply set_add_intro2. reflexivity.
+                    **** crush.
+                         eapply set_add_intro2. reflexivity.
+                +++ clear H0.
 
-                             specialize (address_extend _ _ _ _ _
-                                                        _ _ H1 H5 H2).
-                             intros.
-                             destruct H0.
-                             specialize (mark_ptr_marks x2 h p0 p' H0).
-                             crush.
-                     --- inversion H1. crush. subst.
-                         unfold heap_maps in *. unfold heap_get in *.
-                         rewrite Heqo in H4. discriminate.
-           -- assert (exists v, heap_maps_struct h p'0 v).
-              unfold heap_maps in H2. unfold heap_get in H2.
-              unfold heap_maps_struct. destruct (heap_get_struct p'0 h).
-              crush. exists l. auto. discriminate.
-              destruct H10.
-              specialize (address_extend _ _ _ _ _ _ _ H1 H5 H10).
-              intros.
-              destruct H11.
-              eapply set_union_intro2.
-              eapply mark_ptr_marks.
-              apply H11.
-    - intuition.
-      eapply (FollowAddresses (sweep h (mark r h)) p p'0 p' n address).
-      + clear - H0 H5.
-        remember (mark r h) as foo. clear Heqfoo.
-        induction h. crush.
-        destruct a.
-        unfold sweep in * ; fold sweep in *.
-        unfold heap_maps in * ; fold heap_maps in *.
-        unfold heap_get in * ; fold heap_get in *.
-        unfold heap_get_struct in * ; fold heap_get_struct in *.
-        destruct (ptr_eq_dec p0 p) eqn:?.
-        ** crush.
-           assert (set_mem ptr_eq_dec p foo = true). eapply set_mem_correct2. auto.
-           rewrite H. crush.
-        ** crush.
-           destruct (set_mem ptr_eq_dec p0 foo).
-           -- crush.
-           -- crush.
-      + crush.
+                    specialize (address_extend _ _ _ _ _
+                                               _ _ H1 H5 H2).
+                    intros.
+                    destruct H0.
+                    specialize (mark_ptr_marks x2 h p0 p' H0).
+                    crush.
+            --- inversion H1. crush. subst.
+                unfold heap_maps in *. unfold heap_get in *.
+                rewrite Heqo in H4. discriminate.
+      -- assert (exists v, heap_maps_struct h p'0 v).
+         unfold heap_maps in H2. unfold heap_get in H2.
+         unfold heap_maps_struct. destruct (heap_get_struct p'0 h).
+         crush. exists l. auto. discriminate.
+         destruct H10.
+         specialize (address_extend _ _ _ _ _ _ _ H1 H5 H10).
+         intros.
+         destruct H11.
+         eapply set_union_intro2.
+         eapply mark_ptr_marks.
+         apply H11.
+  - intuition.
+    eapply (FollowAddresses (sweep h (mark r h)) p p'0 p' n address).
+    + clear - H0 H5.
+      remember (mark r h) as foo. clear Heqfoo.
+      induction h. crush.
+      destruct a.
+      unfold sweep in * ; fold sweep in *.
+      unfold heap_maps in * ; fold heap_maps in *.
+      unfold heap_get in * ; fold heap_get in *.
+      unfold heap_get_struct in * ; fold heap_get_struct in *.
+      destruct (ptr_eq_dec p0 p) eqn:?.
+      ** crush.
+         assert (set_mem ptr_eq_dec p foo = true). eapply set_mem_correct2. auto.
+         rewrite H. crush.
+      ** crush.
+         destruct (set_mem ptr_eq_dec p0 foo).
+      -- crush.
+      -- crush.
+    + crush.
 Qed.
 
 Lemma pointer_equivalence :
@@ -561,18 +870,6 @@ Proof.
   * apply H1.
   * unfold heap_maps in H1. unfold heap_get in H1.
     destruct (heap_get_struct p h) eqn:?.
-    - exists l. crush.
-    - crush.
+  - exists l. crush.
+  - crush.
 Qed.
-
-(*
-Theorem safety_1 :
-  forall c s s' s'',
-  small_step c s = Some s' ->
-  small_step c (gc s) = Some s''.
-Proof.
-  intros.
-  destruct c ; unfold small_step in * ; crush.
-  * unfold small_step in H.
-Qed.
-*)
